cedar-lean/Cedar/Thm/Validation.lean
@@ -53,7 +53,7 @@ theorem validation_is_sound (policies : Policies) (schema : Schema) (request : R
   AllEvaluateToBool policies request entities
 := by
   intro hwf h₀ h₁ h₂
-  have h₁ := request_and_entities_validate_implies_match_schema schema request entities hwf h₁ h₂
+  have h₁ := request_and_entities_validate_implies_instance_of_wf_schema schema request entities hwf h₁ h₂
   unfold validate at h₀
   simp only [AllEvaluateToBool]
   cases h₃ : policies with
@@ -91,7 +91,7 @@ theorem validate_with_level_is_sound {ps : Policies} {schema : Schema} {n : Nat}
   isAuthorized request entities ps = isAuthorized request slice ps
 := by
   have hsound : ∀ p ∈ ps, evaluate p.toExpr request entities = evaluate p.toExpr request slice := by
-    have hre := request_and_entities_validate_implies_match_schema _ _ _ hwf hr he
+    have hre := request_and_entities_validate_implies_instance_of_wf_schema _ _ _ hwf hr he
     replace htl := List.forM_ok_implies_all_ok _ _ htl
     intro p hp
     exact typecheck_policy_at_level_with_environments_is_sound hs hre (htl p hp)
